Remove FormalCircuitWithInteractions

Clean/Circuit/StructuralLemmas.lean
@@ -101,36 +101,39 @@ lemma FormalCircuit.weakenSpec_assumptions {F Input Output} [Field F] [ProvableT
   simp only [FormalCircuit.weakenSpec]
 
 /--
-Weaken the specification of a FormalCircuitWithInteractions.
+Weaken the specification of a GeneralFormalCircuit.
 -/
-def FormalCircuitWithInteractions.weakenSpec
+def GeneralFormalCircuit.weakenSpec
     {F : Type} [Field F]
     {Input Output : TypeMap} [ProvableType Input] [ProvableType Output]
-    (circuit : FormalCircuitWithInteractions F Input Output)
-    (WeakerSpec : Input F → Output F → Environment F → Prop)
+    (circuit : GeneralFormalCircuit F Input Output)
+    (WeakerSpec : Input F → Output F → ProverData F → Prop)
     (h_spec_implication : ∀ input output data,
       circuit.Spec input output data → WeakerSpec input output data) :
-    FormalCircuitWithInteractions F Input Output where
+    GeneralFormalCircuit F Input Output where
   __ := circuit.elaborated
   Assumptions := circuit.Assumptions
   Spec := WeakerSpec
   ProverAssumptions := circuit.ProverAssumptions
+  ProverSpec := circuit.ProverSpec
   soundness := by
     intro offset env input_var input h_eval h_assumptions h_holds
     have h_strong_spec := circuit.soundness offset env input_var input h_eval h_assumptions h_holds
     exact ⟨ h_spec_implication input _ _ h_strong_spec.1, h_strong_spec.2 ⟩
   completeness := circuit.completeness
   channelsWithGuarantees := circuit.channelsWithGuarantees
-  guarantees_iff := circuit.guarantees_iff
+  guarantees_in_declared_channels := circuit.guarantees_in_declared_channels
   channelsWithRequirements := circuit.channelsWithRequirements
-  requirements_iff := circuit.requirements_iff
-  shallowChannels_subset := circuit.shallowChannels_subset
+  requirements_in_declared_channels := circuit.requirements_in_declared_channels
+  used_channels_declared := circuit.used_channels_declared
+  exposedChannels := circuit.exposedChannels
+  exposedChannels_eq := circuit.exposedChannels_eq
 
 @[circuit_norm]
-lemma FormalCircuitWithInteractions.weakenSpec_assumptions
+lemma GeneralFormalCircuit.weakenSpec_assumptions
     {F Input Output} [Field F] [ProvableType Input] [ProvableType Output]
-    (c : FormalCircuitWithInteractions F Input Output)
-    (WeakerSpec : Input F → Output F → Environment F → Prop)
+    (c : GeneralFormalCircuit F Input Output)
+    (WeakerSpec : Input F → Output F → ProverData F → Prop)
     h_spec_implication :
     (c.weakenSpec WeakerSpec h_spec_implication).Assumptions = c.Assumptions := by
-  simp only [FormalCircuitWithInteractions.weakenSpec]
+  simp only [GeneralFormalCircuit.weakenSpec]
